YLM: defined+implemented YLM.Sessions module

yahalom/YLM.Sessions.fst
@@ -1,1 +1,96 @@
 module YLM.Sessions
+
+
+let serialize_session_st i p si vi st =
+  let l = readers [V p si vi] in
+  match st with
+  | AuthServerSession pri k_pri_srv ->
+    let tag = M.str_to_bytes #i "srv_sess" in
+    let pri_bytes = M.str_to_bytes #i pri in
+    LC.can_flow_transitive i (LC.get_label M.ylm_key_usages k_pri_srv) (readers [P p]) l;
+    assert(M.is_msg i k_pri_srv l); // required
+    M.concat #i #l tag (M.concat #i #l pri_bytes k_pri_srv)
+  | PKeySession srv k_ps ->
+    let tag = M.str_to_bytes #i "p_key_sess" in
+    let srv_bytes = M.str_to_bytes #i srv in
+    M.concat #i #l tag (M.concat #i #l srv_bytes k_ps)
+  | InitiatorSentMsg1 b n_a ->
+    let tag = M.str_to_bytes #i "i_sent_m1" in
+    let b_bytes = M.str_to_bytes #i b in
+    M.concat #i #l tag (M.concat #i #l b_bytes n_a)
+  | ResponderSentMsg2 a srv n_b ->
+    let tag = M.str_to_bytes #i "r_sent_m2" in
+    let a_bytes = M.str_to_bytes #i a in
+    let srv_bytes = M.str_to_bytes #i srv in
+    M.concat #i #l tag (M.concat #i #l a_bytes (M.concat #i #l srv_bytes n_b))
+  | AuthServerSentMsg3 a b k_ab ->
+    let tag = M.str_to_bytes #i "srv_sent_m3" in
+    let a_bytes = M.str_to_bytes #i a in
+    let b_bytes = M.str_to_bytes #i b in
+    M.concat #i #l tag (M.concat #i #l a_bytes (M.concat #i #l b_bytes k_ab))
+  | InitiatorSentMsg4 b srv k_ab ->
+    let tag = M.str_to_bytes #i "i_sent_m4" in
+    let b_bytes = M.str_to_bytes #i b in
+    let srv_bytes = M.str_to_bytes #i srv in
+    LC.can_flow_transitive i (LC.get_label M.ylm_key_usages k_ab) (readers [P p]) l;
+    M.concat #i #l tag (M.concat #i #l b_bytes (M.concat #i #l srv_bytes k_ab))
+  | ResponderRecvedMsg4 a srv k_ab ->
+    let tag = M.str_to_bytes #i "r_rcvd_m4" in
+    let a_bytes = M.str_to_bytes #i a in
+    let srv_bytes = M.str_to_bytes #i srv in
+    LC.can_flow_transitive i (LC.get_label M.ylm_key_usages k_ab) (readers [P p]) l;
+    M.concat #i #l tag (M.concat #i #l a_bytes (M.concat #i #l srv_bytes k_ab))
+
+let parse_session_st sst =
+  split sst `bind` (fun (tag_bytes, rest) ->
+  bytes_to_string tag_bytes `bind` (fun tag ->
+  match tag with
+  | "srv_sess" ->
+    split rest `bind` (fun (p_bytes, k_ps) ->
+    bytes_to_string p_bytes `bind` (fun p ->
+    Success (AuthServerSession p k_ps)))
+  | "p_key_sess" ->
+    split rest `bind` (fun (srv_bytes, k_ps) ->
+    bytes_to_string srv_bytes `bind` (fun srv ->
+    Success (PKeySession srv k_ps)))
+  | "i_sent_m1" ->
+    split rest `bind` (fun (b_bytes, n_a) ->
+    bytes_to_string b_bytes `bind` (fun b ->
+    Success (InitiatorSentMsg1 b n_a)))
+  | "r_sent_m2" ->
+    split rest `bind` (fun (a_bytes, rest) ->
+    split rest `bind` (fun (srv_bytes, n_b) ->
+    bytes_to_string a_bytes `bind` (fun a ->
+    bytes_to_string srv_bytes `bind` (fun srv ->
+    Success (ResponderSentMsg2 a srv n_b)))))
+  | "srv_sent_m3" ->
+    split rest `bind` (fun (a_bytes, rest) ->
+    split rest `bind` (fun (b_bytes, k_ab) ->
+    bytes_to_string a_bytes `bind` (fun a ->
+    bytes_to_string b_bytes `bind` (fun b ->
+    Success (AuthServerSentMsg3 a b k_ab)))))
+  | "i_sent_m4" ->
+    split rest `bind` (fun (b_bytes, rest) ->
+    split rest `bind` (fun (srv_bytes, k_ab) ->
+    bytes_to_string b_bytes `bind` (fun b ->
+    bytes_to_string srv_bytes `bind` (fun srv ->
+    Success (InitiatorSentMsg4 b srv k_ab)))))
+  | "r_rcvd_m4" ->
+    split rest `bind` (fun (a_bytes, rest) ->
+    split rest `bind` (fun (srv_bytes, k_ab) ->
+    bytes_to_string a_bytes `bind` (fun a ->
+    bytes_to_string srv_bytes `bind` (fun srv ->
+    Success (ResponderRecvedMsg4 a srv k_ab)))))
+  | t -> Error ("[parse_session_st] invalid tag: " ^ t)
+  ))
+
+let parse_serialize_session_st_lemma i p si vi st =
+  let l = readers [V p si vi] in
+  match st with
+  | AuthServerSession pri k_pri_srv ->
+    LC.can_flow_transitive i (LC.get_label M.ylm_key_usages k_pri_srv) (readers [P p]) l
+  | InitiatorSentMsg4 b srv k_ab ->
+    LC.can_flow_transitive i (LC.get_label M.ylm_key_usages k_ab) (readers [P p]) l
+  | ResponderRecvedMsg4 a srv k_ab ->
+    LC.can_flow_transitive i (LC.get_label M.ylm_key_usages k_ab) (readers [P p]) l
+  | _ -> ()
