yahalom/YLM.Sessions.fsti
@@ -1,1 +1,79 @@
 module YLM.Sessions
+
+
+open SecrecyLabels
+open CryptoLib
+
+module M = YLM.Messages
+module LC = LabeledCryptoAPI
+module LR = LabeledRuntimeAPI
+
+
+(* Yahalom specific aliases *)
+
+let is_labeled i b l = LC.is_labeled M.ylm_global_usage i b l
+let is_lt_key i b p srv = LC.is_aead_key M.ylm_global_usage i b (readers [P p; P srv]) "YLM.lt_key"
+let is_comm_key i b srv p q = LC.is_aead_key M.ylm_global_usage i b (readers [P srv; P p; P q]) "YLM.comm_key"
+
+noeq type session_st =
+  (* Auth server session for secret keys shared with principals *)
+  | AuthServerSession: p:principal -> k_ps:bytes -> session_st
+  (* Principal secret key session with auth server *)
+  | PKeySession: srv:principal -> k_ps:bytes -> session_st
+  (* Protocol states *)
+  | InitiatorSentMsg1: b:principal -> n_a:bytes -> session_st
+  | ResponderSentMsg2: a:principal -> srv:principal -> n_b:bytes -> session_st
+  | AuthServerSentMsg3: a:principal -> b:principal -> k_ab:bytes -> session_st
+  | InitiatorSentMsg4: b:principal -> srv:principal -> k_ab:bytes -> session_st
+  | ResponderRecvedMsg4: a:principal -> srv:principal -> k_ab:bytes -> session_st
+
+let valid_session (i:nat) (p:principal) (si vi:nat) (st:session_st) =
+  match st with
+  | AuthServerSession pri k_pri_srv ->
+    M.is_msg i k_pri_srv (readers [P p]) /\ is_lt_key i k_pri_srv pri p
+  | PKeySession srv k_ps -> is_lt_key i k_ps p srv
+  | InitiatorSentMsg1 b n_a -> is_labeled i n_a public
+  | ResponderSentMsg2 a srv n_b -> is_labeled i n_b (readers [P p; P a; P srv])
+  | AuthServerSentMsg3 a b k_ab -> is_comm_key i k_ab p a b
+  | InitiatorSentMsg4 b srv k_ab ->
+    M.is_msg i k_ab (readers [P p]) /\
+    (is_labeled i k_ab (readers [P srv; P p; P b]) \/ LC.corrupt_id i (P srv) \/ LC.corrupt_id i (P p) \/ LC.corrupt_id i (P b))
+  | ResponderRecvedMsg4 a srv k_ab ->
+    M.is_msg i k_ab (readers [P p]) /\
+    (is_labeled i k_ab (readers [P srv; P a; P p]) \/ LC.corrupt_id i (P srv) \/ LC.corrupt_id i (P a) \/ LC.corrupt_id i (P p))
+
+let valid_session_later (i j:timestamp) (p:principal) (si vi:nat) (st:session_st) :
+  Lemma (ensures (valid_session i p si vi st /\ later_than j i ==> valid_session j p si vi st))
+= ()
+
+val serialize_session_st: i:nat -> p:principal -> si:nat -> vi:nat -> st:session_st{valid_session i p si vi st} -> M.msg i (readers [V p si vi])
+
+val parse_session_st: sst:bytes -> result session_st
+
+val parse_serialize_session_st_lemma: i:nat -> p:principal -> si:nat -> vi:nat -> st:session_st ->
+    Lemma (requires (valid_session i p si vi st))
+	  (ensures  (Success st == parse_session_st (serialize_session_st i p si vi st)))
+	  [SMTPat (parse_session_st (serialize_session_st i p si vi st))]
+
+
+let epred idx s e = True
+
+let ylm_session_st_inv (trace_idx:nat) (p:principal) (state_session_idx:nat) (version:nat) (state:bytes) =
+    M.is_msg trace_idx state (readers [V p state_session_idx version]) /\
+    (match parse_session_st state with
+     | Success state -> valid_session trace_idx p state_session_idx version state
+     | _ -> True)
+
+let ylm_preds: LR.preds = {
+  LR.global_usage = M.ylm_global_usage;
+  LR.trace_preds = {
+    LR.can_trigger_event = epred;
+    LR.session_st_inv = ylm_session_st_inv;
+    LR.session_st_inv_later = (fun i j p si vi sst ->
+      match parse_session_st sst with
+      | Success st -> valid_session_later i j p si vi st
+      | _ -> ()
+    );
+    LR.session_st_inv_lemma = (fun i p si vi sst -> ())
+  }
+}
